proofs/fstar/extraction/Sandwich.Support.Data_source.fsti
@@ -3,6 +3,14 @@ module Sandwich.Support.Data_source
 open Core
 open FStar.Mul
 
+let _ =
+  (* This module has implicit dependencies, here we make them explicit. *)
+  (* The implicit dependencies arise from typeclasses instances. *)
+  let open Sandwich.Error in
+  let open Sandwich.Error.Code in
+  let open Std.Path in
+  ()
+
 /// A source of data.
 /// Source of the material is either from the local filesystem (`Fs`), from
 /// an inline slice of bytes (`Bytes`) or from a inline string (`String`).
@@ -14,11 +22,27 @@ type t_DataSource =
 
 /// Returns the data holds by the [`DataSource`] as a slice of bytes.
 [@@ FStar.Tactics.Typeclasses.tcinstance]
-val impl_1:Core.Convert.t_AsRef t_DataSource (t_Slice u8)
-
-/// Implements [`std::fmt::Debug`] for [`DataSource`].
-[@@ FStar.Tactics.Typeclasses.tcinstance]
-val impl_2:Core.Fmt.t_Debug t_DataSource
+let impl_1: Core.Convert.t_AsRef t_DataSource (t_Slice u8) =
+  {
+    f_as_ref_pre = (fun (self: t_DataSource) -> true);
+    f_as_ref_post = (fun (self: t_DataSource) (out: t_Slice u8) -> true);
+    f_as_ref
+    =
+    fun (self: t_DataSource) ->
+      match self with
+      | DataSource_Fs v ->
+        Core.Ops.Deref.f_deref #(Alloc.Vec.t_Vec u8 Alloc.Alloc.t_Global)
+          #FStar.Tactics.Typeclasses.solve
+          v
+      | DataSource_Bytes b ->
+        Core.Ops.Deref.f_deref #(Alloc.Borrow.t_Cow (t_Slice u8)) #FStar.Tactics.Typeclasses.solve b
+      | DataSource_String s ->
+        Core.Str.impl__str__as_bytes (Core.Ops.Deref.f_deref #(Alloc.Borrow.t_Cow string)
+              #FStar.Tactics.Typeclasses.solve
+              s
+            <:
+            string)
+  }
 
 /// Instantiates a [`DataSource`] from a protobuf `DataSource` message.
 /// # Errors
@@ -28,4 +52,137 @@ val impl_2:Core.Fmt.t_Debug t_DataSource
 /// If the protobuf `DataSource` message doesn't provide any source type,
 /// then `DataSourceError::DATASOURCEERROR_INVALID_CASE` is returned.
 [@@ FStar.Tactics.Typeclasses.tcinstance]
-val impl:Core.Convert.t_TryFrom t_DataSource Sandwich_api_proto.Data_source.t_DataSource
+let impl: Core.Convert.t_TryFrom t_DataSource Sandwich_api_proto.Data_source.t_DataSource =
+  {
+    f_Error = Sandwich.Error.t_Error;
+    f_try_from_pre = (fun (ds: Sandwich_api_proto.Data_source.t_DataSource) -> true);
+    f_try_from_post
+    =
+    (fun
+        (ds: Sandwich_api_proto.Data_source.t_DataSource)
+        (out: Core.Result.t_Result t_DataSource Sandwich.Error.t_Error)
+        ->
+        true);
+    f_try_from
+    =
+    fun (ds: Sandwich_api_proto.Data_source.t_DataSource) ->
+      Core.Result.impl__and_then #Sandwich_api_proto.Data_source.Data_source.t_Specifier
+        #Sandwich.Error.t_Error
+        #t_DataSource
+        (Core.Option.impl__ok_or_else #Sandwich_api_proto.Data_source.Data_source.t_Specifier
+            #Sandwich.Error.t_Error
+            (Core.Option.impl__as_ref #Sandwich_api_proto.Data_source.Data_source.t_Specifier
+                ds.Sandwich_api_proto.Data_source.f_specifier
+              <:
+              Core.Option.t_Option Sandwich_api_proto.Data_source.Data_source.t_Specifier)
+            (fun temp_0_ ->
+                let _:Prims.unit = temp_0_ in
+                Core.Convert.f_into #Sandwich_proto.Errors.t_DataSourceError
+                  #Sandwich.Error.t_Error
+                  #FStar.Tactics.Typeclasses.solve
+                  (Sandwich_proto.Errors.DataSourceError_DATASOURCEERROR_INVALID_CASE
+                    <:
+                    Sandwich_proto.Errors.t_DataSourceError)
+                <:
+                Sandwich.Error.t_Error)
+          <:
+          Core.Result.t_Result Sandwich_api_proto.Data_source.Data_source.t_Specifier
+            Sandwich.Error.t_Error)
+        (fun oneof ->
+            let oneof:Sandwich_api_proto.Data_source.Data_source.t_Specifier = oneof in
+            match oneof with
+            | Sandwich_api_proto.Data_source.Data_source.Specifier_Filename path ->
+              (match
+                  Core.Result.impl__or #(Alloc.Vec.t_Vec u8 Alloc.Alloc.t_Global)
+                    #Std.Io.Error.t_Error
+                    #Sandwich_proto.Errors.t_DataSourceError
+                    (Std.Fs.read #Alloc.String.t_String path
+                      <:
+                      Core.Result.t_Result (Alloc.Vec.t_Vec u8 Alloc.Alloc.t_Global)
+                        Std.Io.Error.t_Error)
+                    (Core.Result.Result_Err
+                      (Sandwich_proto.Errors.DataSourceError_DATASOURCEERROR_NOT_FOUND
+                        <:
+                        Sandwich_proto.Errors.t_DataSourceError)
+                      <:
+                      Core.Result.t_Result (Alloc.Vec.t_Vec u8 Alloc.Alloc.t_Global)
+                        Sandwich_proto.Errors.t_DataSourceError)
+                  <:
+                  Core.Result.t_Result (Alloc.Vec.t_Vec u8 Alloc.Alloc.t_Global)
+                    Sandwich_proto.Errors.t_DataSourceError
+                with
+                | Core.Result.Result_Ok hoist20 ->
+                  Core.Ops.Control_flow.ControlFlow_Continue
+                  (Core.Result.Result_Ok (DataSource_Fs hoist20 <: t_DataSource)
+                    <:
+                    Core.Result.t_Result t_DataSource Sandwich.Error.t_Error)
+                  <:
+                  Core.Ops.Control_flow.t_ControlFlow
+                    (Core.Result.t_Result t_DataSource Sandwich.Error.t_Error)
+                    (Core.Result.t_Result t_DataSource Sandwich.Error.t_Error)
+                | Core.Result.Result_Err err ->
+                  Core.Ops.Control_flow.ControlFlow_Break
+                  (Core.Result.Result_Err
+                    (Core.Convert.f_from #FStar.Tactics.Typeclasses.solve err
+                      <:
+                      Sandwich_proto.Errors.t_DataSourceError -> Sandwich.Error.t_Error)
+                    <:
+                    Core.Result.t_Result t_DataSource Sandwich.Error.t_Error)
+                  <:
+                  Core.Ops.Control_flow.t_ControlFlow
+                    (Core.Result.t_Result t_DataSource Sandwich.Error.t_Error)
+                    (Core.Result.t_Result t_DataSource Sandwich.Error.t_Error))
+            | Sandwich_api_proto.Data_source.Data_source.Specifier_InlineBytes v ->
+              Core.Ops.Control_flow.ControlFlow_Continue
+              (Core.Result.Result_Ok
+                (DataSource_Bytes
+                  (Core.Convert.f_from #(Alloc.Borrow.t_Cow (t_Slice u8))
+                      #(Alloc.Vec.t_Vec u8 Alloc.Alloc.t_Global)
+                      #FStar.Tactics.Typeclasses.solve
+                      v
+                    <:
+                    Alloc.Borrow.t_Cow (t_Slice u8))
+                  <:
+                  t_DataSource)
+                <:
+                Core.Result.t_Result t_DataSource Sandwich.Error.t_Error)
+              <:
+              Core.Ops.Control_flow.t_ControlFlow
+                (Core.Result.t_Result t_DataSource Sandwich.Error.t_Error)
+                (Core.Result.t_Result t_DataSource Sandwich.Error.t_Error)
+            | Sandwich_api_proto.Data_source.Data_source.Specifier_InlineString v ->
+              Core.Ops.Control_flow.ControlFlow_Continue
+              (Core.Result.Result_Ok
+                (DataSource_String
+                  (Core.Convert.f_from #(Alloc.Borrow.t_Cow string)
+                      #Alloc.String.t_String
+                      #FStar.Tactics.Typeclasses.solve
+                      v
+                    <:
+                    Alloc.Borrow.t_Cow string)
+                  <:
+                  t_DataSource)
+                <:
+                Core.Result.t_Result t_DataSource Sandwich.Error.t_Error)
+              <:
+              Core.Ops.Control_flow.t_ControlFlow
+                (Core.Result.t_Result t_DataSource Sandwich.Error.t_Error)
+                (Core.Result.t_Result t_DataSource Sandwich.Error.t_Error)
+            | _ ->
+              Core.Ops.Control_flow.ControlFlow_Continue
+              (Core.Result.Result_Err
+                (Core.Convert.f_into #Sandwich_proto.Errors.t_DataSourceError
+                    #Sandwich.Error.t_Error
+                    #FStar.Tactics.Typeclasses.solve
+                    (Sandwich_proto.Errors.DataSourceError_DATASOURCEERROR_INVALID_CASE
+                      <:
+                      Sandwich_proto.Errors.t_DataSourceError)
+                  <:
+                  Sandwich.Error.t_Error)
+                <:
+                Core.Result.t_Result t_DataSource Sandwich.Error.t_Error)
+              <:
+              Core.Ops.Control_flow.t_ControlFlow
+                (Core.Result.t_Result t_DataSource Sandwich.Error.t_Error)
+                (Core.Result.t_Result t_DataSource Sandwich.Error.t_Error))
+  }
