proofs/fstar/extraction/Sandwich.Implementation.Openssl3.Error.fst
@@ -1,0 +1,73 @@
+module Sandwich.Implementation.Openssl3.Error
+#set-options "--fuel 0 --ifuel 1 --z3rlimit 15"
+open Core
+open FStar.Mul
+
+let t_ErrorLibrary_cast_to_repr (x: t_ErrorLibrary) =
+  match x with
+  | ErrorLibrary_None  -> discriminant_ErrorLibrary_None
+  | ErrorLibrary_Sys  -> discriminant_ErrorLibrary_Sys
+  | ErrorLibrary_Bn  -> discriminant_ErrorLibrary_Bn
+  | ErrorLibrary_Rsa  -> discriminant_ErrorLibrary_Rsa
+  | ErrorLibrary_Dh  -> discriminant_ErrorLibrary_Dh
+  | ErrorLibrary_Evp  -> discriminant_ErrorLibrary_Evp
+  | ErrorLibrary_Buf  -> discriminant_ErrorLibrary_Buf
+  | ErrorLibrary_Obj  -> discriminant_ErrorLibrary_Obj
+  | ErrorLibrary_Pem  -> discriminant_ErrorLibrary_Pem
+  | ErrorLibrary_Dsa  -> discriminant_ErrorLibrary_Dsa
+  | ErrorLibrary_X509  -> discriminant_ErrorLibrary_X509
+  | ErrorLibrary_Asn1  -> discriminant_ErrorLibrary_Asn1
+  | ErrorLibrary_Conf  -> discriminant_ErrorLibrary_Conf
+  | ErrorLibrary_Crypto  -> discriminant_ErrorLibrary_Crypto
+  | ErrorLibrary_Ec  -> discriminant_ErrorLibrary_Ec
+  | ErrorLibrary_Ssl  -> discriminant_ErrorLibrary_Ssl
+  | ErrorLibrary_Bio  -> discriminant_ErrorLibrary_Bio
+  | ErrorLibrary_Pkcs7  -> discriminant_ErrorLibrary_Pkcs7
+  | ErrorLibrary_X509v3  -> discriminant_ErrorLibrary_X509v3
+  | ErrorLibrary_Pkcs12  -> discriminant_ErrorLibrary_Pkcs12
+  | ErrorLibrary_Rand  -> discriminant_ErrorLibrary_Rand
+  | ErrorLibrary_Dso  -> discriminant_ErrorLibrary_Dso
+  | ErrorLibrary_Engine  -> discriminant_ErrorLibrary_Engine
+  | ErrorLibrary_Ocsp  -> discriminant_ErrorLibrary_Ocsp
+  | ErrorLibrary_Ui  -> discriminant_ErrorLibrary_Ui
+  | ErrorLibrary_Comp  -> discriminant_ErrorLibrary_Comp
+  | ErrorLibrary_Ecdsa  -> discriminant_ErrorLibrary_Ecdsa
+  | ErrorLibrary_Ecdh  -> discriminant_ErrorLibrary_Ecdh
+  | ErrorLibrary_OsslStore  -> discriminant_ErrorLibrary_OsslStore
+  | ErrorLibrary_Fips  -> discriminant_ErrorLibrary_Fips
+  | ErrorLibrary_Cms  -> discriminant_ErrorLibrary_Cms
+  | ErrorLibrary_Ts  -> discriminant_ErrorLibrary_Ts
+  | ErrorLibrary_Hmac  -> discriminant_ErrorLibrary_Hmac
+  | ErrorLibrary_Ct  -> discriminant_ErrorLibrary_Ct
+  | ErrorLibrary_Async  -> discriminant_ErrorLibrary_Async
+  | ErrorLibrary_Kdf  -> discriminant_ErrorLibrary_Kdf
+  | ErrorLibrary_Sm2  -> discriminant_ErrorLibrary_Sm2
+  | ErrorLibrary_Ess  -> discriminant_ErrorLibrary_Ess
+  | ErrorLibrary_Prop  -> discriminant_ErrorLibrary_Prop
+  | ErrorLibrary_Crmf  -> discriminant_ErrorLibrary_Crmf
+  | ErrorLibrary_Prov  -> discriminant_ErrorLibrary_Prov
+  | ErrorLibrary_Cmp  -> discriminant_ErrorLibrary_Cmp
+  | ErrorLibrary_OsslEncoder  -> discriminant_ErrorLibrary_OsslEncoder
+  | ErrorLibrary_OsslDecoder  -> discriminant_ErrorLibrary_OsslDecoder
+  | ErrorLibrary_Http  -> discriminant_ErrorLibrary_Http
+  | ErrorLibrary_User  -> discriminant_ErrorLibrary_User
+
+let t_SslError_cast_to_repr (x: t_SslError) =
+  match x with
+  | SslError_None  -> discriminant_SslError_None
+  | SslError_Ssl  -> discriminant_SslError_Ssl
+  | SslError_WantRead  -> discriminant_SslError_WantRead
+  | SslError_WantWrite  -> discriminant_SslError_WantWrite
+  | SslError_WantX509Lookup  -> discriminant_SslError_WantX509Lookup
+  | SslError_Syscall  -> discriminant_SslError_Syscall
+  | SslError_ZeroReturn  -> discriminant_SslError_ZeroReturn
+  | SslError_WantConnect  -> discriminant_SslError_WantConnect
+  | SslError_WantAccept  -> discriminant_SslError_WantAccept
+  | SslError_WantAsync  -> discriminant_SslError_WantAsync
+  | SslError_WantAsyncJob  -> discriminant_SslError_WantAsyncJob
+  | SslError_WantClientHelloCb  -> discriminant_SslError_WantClientHelloCb
+  | SslError_WantRetryVerify  -> discriminant_SslError_WantRetryVerify
+
+let impl__Error__library (self: t_Error) = self.f_library
+
+let impl__Error__reason (self: t_Error) = cast (self.f_reason <: i32) <: u32
