proofs/fstar/extraction/Sandwich.Implementation.Openssl3.Tunnel.Ssl.fsti
@@ -1,0 +1,356 @@
+module Sandwich.Implementation.Openssl3.Tunnel.Ssl
+#set-options "--fuel 0 --ifuel 1 --z3rlimit 15"
+open Core
+open FStar.Mul
+
+let _ =
+  (* This module has implicit dependencies, here we make them explicit. *)
+  (* The implicit dependencies arise from typeclasses instances. *)
+  let open Sandwich.Error in
+  let open Sandwich.Error.Code in
+  let open Sandwich.Implementation.Openssl3.Error in
+  let open Sandwich.Implementation.Openssl3.Tunnel.X509_verify_param in
+  let open Sandwich.Tunnel in
+  let open Sandwich.Tunnel.Tls in
+  let open Sandwich_proto.Tunnel in
+  ()
+
+/// Index in the SSL user data (`SSL_get_ex_data`/`SSL_set_ex_data`) where
+/// the pointer to the tunnel security requirements is stored.
+let v_SSL_EX_DATA_TUNNEL_SECURITY_REQUIREMENTS_INDEX: i32 = 1l
+
+/// Wrapper of the OpenSSL SSL object.
+type t_Ssl = | Ssl : Core.Ptr.Non_null.t_NonNull Openssl3.t_ssl_st -> t_Ssl
+
+[@@ FStar.Tactics.Typeclasses.tcinstance]
+let impl: Core.Fmt.t_Debug t_Ssl =
+  {
+    f_fmt_pre = (fun (self: t_Ssl) (f: Core.Fmt.t_Formatter) -> true);
+    f_fmt_post
+    =
+    (fun
+        (self: t_Ssl)
+        (f: Core.Fmt.t_Formatter)
+        (out1: (Core.Fmt.t_Formatter & Core.Result.t_Result Prims.unit Core.Fmt.t_Error))
+        ->
+        true);
+    f_fmt
+    =
+    fun (self: t_Ssl) (f: Core.Fmt.t_Formatter) ->
+      let tmp0, out:(Core.Fmt.t_Formatter & Core.Result.t_Result Prims.unit Core.Fmt.t_Error) =
+        Core.Fmt.impl_7__write_fmt f
+          (Core.Fmt.impl_2__new_v1 (sz 2)
+              (sz 1)
+              (let list = ["OpenSSL3SSLObject("; ")"] in
+                FStar.Pervasives.assert_norm (Prims.eq2 (List.Tot.length list) 2);
+                Rust_primitives.Hax.array_of_list 2 list)
+              (let list =
+                  [
+                    Core.Fmt.Rt.impl_1__new_pointer #(Core.Ptr.Non_null.t_NonNull Openssl3.t_ssl_st)
+                      self._0
+                    <:
+                    Core.Fmt.Rt.t_Argument
+                  ]
+                in
+                FStar.Pervasives.assert_norm (Prims.eq2 (List.Tot.length list) 1);
+                Rust_primitives.Hax.array_of_list 1 list)
+            <:
+            Core.Fmt.t_Arguments)
+      in
+      let f:Core.Fmt.t_Formatter = tmp0 in
+      let hax_temp_output:Core.Result.t_Result Prims.unit Core.Fmt.t_Error = out in
+      f, hax_temp_output
+      <:
+      (Core.Fmt.t_Formatter & Core.Result.t_Result Prims.unit Core.Fmt.t_Error)
+  }
+
+[@@ FStar.Tactics.Typeclasses.tcinstance]
+let impl_1: Core.Convert.t_From t_Ssl (Core.Ptr.Non_null.t_NonNull Openssl3.t_ssl_st) =
+  {
+    f_from_pre = (fun (ssl: Core.Ptr.Non_null.t_NonNull Openssl3.t_ssl_st) -> true);
+    f_from_post = (fun (ssl: Core.Ptr.Non_null.t_NonNull Openssl3.t_ssl_st) (out: t_Ssl) -> true);
+    f_from = fun (ssl: Core.Ptr.Non_null.t_NonNull Openssl3.t_ssl_st) -> Ssl ssl <: t_Ssl
+  }
+
+/// Returns a pointer to the BIO currently attached to the SSL object.
+val impl__Ssl__get_attached_bio (self: t_Ssl)
+    : Prims.Pure (Core.Option.t_Option (Core.Ptr.Non_null.t_NonNull Openssl3.t_bio_st))
+      Prims.l_True
+      (fun _ -> Prims.l_True)
+
+/// Returns a pointer to some extra data from a SSL object.
+val impl__Ssl__get_extra_data_ptr
+      (#v_T #impl_765196419_: Type0)
+      {| i2: Core.Convert.t_Into impl_765196419_ i32 |}
+      (self: t_Ssl)
+      (extra_data_index: impl_765196419_)
+    : Prims.Pure (Core.Option.t_Option (Core.Ptr.Non_null.t_NonNull v_T))
+      Prims.l_True
+      (fun _ -> Prims.l_True)
+
+/// Returns a reference to some extra data from a SSL object.
+val impl__Ssl__get_extra_data_ref
+      (#v_T #impl_765196419_: Type0)
+      {| i5: Core.Convert.t_Into impl_765196419_ i32 |}
+      (self: t_Ssl)
+      (extra_data_index: impl_765196419_)
+    : Prims.Pure (Core.Option.t_Option v_T) Prims.l_True (fun _ -> Prims.l_True)
+
+/// Returns the last recorded error.
+val impl__Ssl__get_last_recorded_error
+      (#impl_765196419_: Type0)
+      {| i7: Core.Convert.t_Into impl_765196419_ i32 |}
+      (self: t_Ssl)
+      (ret: impl_765196419_)
+    : Prims.Pure (Core.Result.t_Result Sandwich.Implementation.Openssl3.Error.t_SslError i32)
+      Prims.l_True
+      (fun _ -> Prims.l_True)
+
+/// Returns the error that occurred during the record stage.
+/// The record stage is the stage when `SSL_read` and `SSL_write`
+/// are called.
+val impl__Ssl__get_error_from_record_stage (self: t_Ssl) (err: i32)
+    : Prims.Pure Sandwich_proto.Tunnel.t_RecordError Prims.l_True (fun _ -> Prims.l_True)
+
+/// Returns the state of the SSL tunnel.
+val impl__Ssl__get_state (self: t_Ssl)
+    : Prims.Pure Sandwich_proto.Tunnel.t_HandshakeState Prims.l_True (fun _ -> Prims.l_True)
+
+/// Checks if the tunnel is in a shutdown state.
+val impl__Ssl__is_shutdown (self: t_Ssl) : Prims.Pure bool Prims.l_True (fun _ -> Prims.l_True)
+
+/// Returns the tunnel security requirements from a SSL object.
+val impl__Ssl__get_tunnel_security_requirements (self: t_Ssl)
+    : Prims.Pure (Core.Option.t_Option Sandwich.Tunnel.Tls.t_TunnelSecurityRequirements)
+      Prims.l_True
+      (fun _ -> Prims.l_True)
+
+/// Creates a new Sandwich BIO and attach it to the SSL object.
+val impl__Ssl__create_and_attach_bio (self: t_Ssl)
+    : Prims.Pure (Core.Result.t_Result Prims.unit Sandwich.Error.t_Error)
+      Prims.l_True
+      (fun _ -> Prims.l_True)
+
+/// Handles an SSL error of type `SSL_ERROR_SSL`.
+val impl__Ssl__handle_ssl_error_ssl (self: t_Ssl)
+    : Prims.Pure
+      (Core.Result.t_Result Sandwich_proto.Tunnel.t_HandshakeState Sandwich.Error.t_Error &
+        Core.Option.t_Option Sandwich_proto.Tunnel.t_State) Prims.l_True (fun _ -> Prims.l_True)
+
+/// Performs the handshake.
+val impl__Ssl__do_handshake (self: t_Ssl)
+    : Prims.Pure
+      (Core.Result.t_Result Sandwich_proto.Tunnel.t_HandshakeState Sandwich.Error.t_Error &
+        Core.Option.t_Option Sandwich_proto.Tunnel.t_State) Prims.l_True (fun _ -> Prims.l_True)
+
+/// Sets the server name indication (SNI).
+val impl__Ssl__set_server_name_indication
+      (#impl_488124255_: Type0)
+      {| i9: Core.Convert.t_AsRef impl_488124255_ string |}
+      (self: t_Ssl)
+      (sni: impl_488124255_)
+    : Prims.Pure (Core.Result.t_Result Prims.unit Sandwich.Error.t_Error)
+      Prims.l_True
+      (fun _ -> Prims.l_True)
+
+/// Verifies the tunnel configuration against the security requirements that come
+/// from the context.
+val verify_tunnel_verifier
+      (tunnel_verifier: Core.Option.t_Option Sandwich_api_proto.Verifiers.t_TunnelVerifier)
+      (security_requirements: Sandwich.Tunnel.Tls.t_TunnelSecurityRequirements)
+    : Prims.Pure (Core.Result.t_Result Prims.unit Sandwich.Error.t_Error)
+      Prims.l_True
+      (fun _ -> Prims.l_True)
+
+/// Sets the required Subject Alternative Names (SAN) specified in the [`pb_api::TunnelVerifier`]
+/// object.
+val impl__Ssl__set_subject_alternative_names
+      (self: t_Ssl)
+      (tunnel_verifier: Core.Option.t_Option Sandwich_api_proto.Verifiers.t_TunnelVerifier)
+    : Prims.Pure (Core.Result.t_Result Prims.unit Sandwich.Error.t_Error)
+      Prims.l_True
+      (fun _ -> Prims.l_True)
+
+/// Closes the tunnel.
+val impl__Ssl__close (self: t_Ssl)
+    : Prims.Pure
+      (Core.Result.t_Result Prims.unit
+          (Sandwich.Tunnel.t_ProtoStateErrorBase Sandwich_proto.Tunnel.t_RecordError))
+      Prims.l_True
+      (fun _ -> Prims.l_True)
+
+/// Reads some data and writes it to a buffer.
+val impl__Ssl__read (self: t_Ssl) (buffer: t_Slice u8)
+    : Prims.Pure
+      (t_Slice u8 &
+        Core.Result.t_Result usize
+          (Sandwich.Tunnel.t_ProtoStateErrorBase Sandwich_proto.Tunnel.t_RecordError))
+      Prims.l_True
+      (fun _ -> Prims.l_True)
+
+/// Write some data.
+val impl__Ssl__write (self: t_Ssl) (buffer: t_Slice u8)
+    : Prims.Pure
+      (Core.Result.t_Result usize
+          (Sandwich.Tunnel.t_ProtoStateErrorBase Sandwich_proto.Tunnel.t_RecordError))
+      Prims.l_True
+      (fun _ -> Prims.l_True)
+
+/// A tunnel, wrapper around a SSL object.
+type t_Tunnel = {
+  f__ssl_ctx:Sandwich.Implementation.Openssl3.Tunnel.Context.t_Context;
+  f_ssl:Sandwich.Support.Pimpl.t_Pimpl Openssl3.t_ssl_st;
+  f_security_requirements:Sandwich.Tunnel.Tls.t_TunnelSecurityRequirements;
+  f_io:Sandwich.Tunnel.Io.t_BoxedIO;
+  f_state:Sandwich_proto.Tunnel.t_State
+}
+
+[@@ FStar.Tactics.Typeclasses.tcinstance]
+let impl_3: Core.Fmt.t_Debug t_Tunnel =
+  {
+    f_fmt_pre = (fun (self: t_Tunnel) (f: Core.Fmt.t_Formatter) -> true);
+    f_fmt_post
+    =
+    (fun
+        (self: t_Tunnel)
+        (f: Core.Fmt.t_Formatter)
+        (out1: (Core.Fmt.t_Formatter & Core.Result.t_Result Prims.unit Core.Fmt.t_Error))
+        ->
+        true);
+    f_fmt
+    =
+    fun (self: t_Tunnel) (f: Core.Fmt.t_Formatter) ->
+      let tmp0, out:(Core.Fmt.t_Formatter & Core.Result.t_Result Prims.unit Core.Fmt.t_Error) =
+        Core.Fmt.impl_7__write_fmt f
+          (Core.Fmt.impl_2__new_v1 (sz 2)
+              (sz 1)
+              (let list = ["OpenSSL3Tunnel(ssl: "; ")"] in
+                FStar.Pervasives.assert_norm (Prims.eq2 (List.Tot.length list) 2);
+                Rust_primitives.Hax.array_of_list 2 list)
+              (let list =
+                  [
+                    Rust_primitives.Hax.failure "(reject_RawOrMutPointer) ExplicitRejection { reason: \"a node of kind [Raw_pointer] have been found in the AST\" }"
+                      "core::fmt::rt::impl_1__new_pointer::<\n        lifetime!(something),\n        raw_pointer!(),\n    >(\n        &(deref(\n            &(core::ptr::non_null::impl_3__as_ptr::<\n                openssl3::t_ssl_st,\n            >(\n                sandwich::support::pimpl::impl_2__as_nonnull::<\n                    lifetime!(something),\n                    openssl3::t_ssl_st,\n                >(\n                    &(proj_sandwich::implementation::openssl3::tunnel::ssl::f_ssl(\n                        deref(self),\n                    )),\n                ),\n            )),\n        )),\n    )"
+
+                    <:
+                    Core.Fmt.Rt.t_Argument
+                  ]
+                in
+                FStar.Pervasives.assert_norm (Prims.eq2 (List.Tot.length list) 1);
+                Rust_primitives.Hax.array_of_list 1 list)
+            <:
+            Core.Fmt.t_Arguments)
+      in
+      let f:Core.Fmt.t_Formatter = tmp0 in
+      let hax_temp_output:Core.Result.t_Result Prims.unit Core.Fmt.t_Error = out in
+      f, hax_temp_output
+      <:
+      (Core.Fmt.t_Formatter & Core.Result.t_Result Prims.unit Core.Fmt.t_Error)
+  }
+
+/// Attaches the security requirements structure to the `SSL` object
+/// through `ex_data`.
+val impl_6__attach_security_requirements (self: Core.Pin.t_Pin t_Tunnel)
+    : Prims.Pure (Core.Result.t_Result Prims.unit Sandwich.Error.t_Error)
+      Prims.l_True
+      (fun _ -> Prims.l_True)
+
+/// Attaches itself to the current BIO.
+val impl_6__attach_to_bio (self: Core.Pin.t_Pin t_Tunnel)
+    : Prims.Pure (Core.Result.t_Result Prims.unit Sandwich.Error.t_Error)
+      Prims.l_True
+      (fun _ -> Prims.l_True)
+
+val impl_6__handshake (self: t_Tunnel)
+    : Prims.Pure
+      (t_Tunnel &
+        Core.Result.t_Result
+          (Sandwich.Tunnel.t_ProtoStateErrorBase Sandwich_proto.Tunnel.t_HandshakeState)
+          Sandwich.Error.t_Error) Prims.l_True (fun _ -> Prims.l_True)
+
+val impl_6__state (self: t_Tunnel)
+    : Prims.Pure (Sandwich.Tunnel.t_ProtoStateErrorBase Sandwich_proto.Tunnel.t_State)
+      Prims.l_True
+      (fun _ -> Prims.l_True)
+
+/// Updates the state of the tunnel.
+/// This method must be called after any read or write operation.
+val impl_6__update_state (self: t_Tunnel) : Prims.Pure t_Tunnel Prims.l_True (fun _ -> Prims.l_True)
+
+val impl_6__close (self: t_Tunnel)
+    : Prims.Pure
+      (t_Tunnel &
+        Core.Result.t_Result Prims.unit
+          (Sandwich.Tunnel.t_ProtoStateErrorBase Sandwich_proto.Tunnel.t_RecordError))
+      Prims.l_True
+      (fun _ -> Prims.l_True)
+
+val impl_6__read (self: t_Tunnel) (buf: t_Slice u8)
+    : Prims.Pure
+      (t_Slice u8 &
+        (t_Tunnel &
+          Core.Result.t_Result usize
+            (Sandwich.Tunnel.t_ProtoStateErrorBase Sandwich_proto.Tunnel.t_RecordError)))
+      Prims.l_True
+      (fun _ -> Prims.l_True)
+
+val impl_6__write (self: t_Tunnel) (buf: t_Slice u8)
+    : Prims.Pure
+      (t_Tunnel &
+        Core.Result.t_Result usize
+          (Sandwich.Tunnel.t_ProtoStateErrorBase Sandwich_proto.Tunnel.t_RecordError))
+      Prims.l_True
+      (fun _ -> Prims.l_True)
+
+/// Tunnel builder.
+/// This is a convenient aggregate of useful values to build a tunnel.
+type t_TunnelBuilder = {
+  f_ssl_ctx:Sandwich.Implementation.Openssl3.Tunnel.Context.t_Context;
+  f_io:Sandwich.Tunnel.Io.t_BoxedIO;
+  f_configuration:Sandwich_api_proto.Tunnel.t_TunnelConfiguration
+}
+
+[@@ FStar.Tactics.Typeclasses.tcinstance]
+let impl_4: Core.Fmt.t_Debug t_TunnelBuilder =
+  {
+    f_fmt_pre = (fun (self: t_TunnelBuilder) (f: Core.Fmt.t_Formatter) -> true);
+    f_fmt_post
+    =
+    (fun
+        (self: t_TunnelBuilder)
+        (f: Core.Fmt.t_Formatter)
+        (out1: (Core.Fmt.t_Formatter & Core.Result.t_Result Prims.unit Core.Fmt.t_Error))
+        ->
+        true);
+    f_fmt
+    =
+    fun (self: t_TunnelBuilder) (f: Core.Fmt.t_Formatter) ->
+      let tmp0, out:(Core.Fmt.t_Formatter & Core.Result.t_Result Prims.unit Core.Fmt.t_Error) =
+        Core.Fmt.impl_7__write_fmt f
+          (Core.Fmt.impl_2__new_const (sz 1)
+              (let list = ["OpenSSL3TunnelBuilder"] in
+                FStar.Pervasives.assert_norm (Prims.eq2 (List.Tot.length list) 1);
+                Rust_primitives.Hax.array_of_list 1 list)
+            <:
+            Core.Fmt.t_Arguments)
+      in
+      let f:Core.Fmt.t_Formatter = tmp0 in
+      let hax_temp_output:Core.Result.t_Result Prims.unit Core.Fmt.t_Error = out in
+      f, hax_temp_output
+      <:
+      (Core.Fmt.t_Formatter & Core.Result.t_Result Prims.unit Core.Fmt.t_Error)
+  }
+
+/// Prepares a tunnel structure.
+val impl_5__prepare_ssl (self: t_TunnelBuilder)
+    : Prims.Pure
+      (Core.Result.t_Result (Sandwich.Support.Pimpl.t_Pimpl Openssl3.t_ssl_st)
+          Sandwich.Error.t_Error) Prims.l_True (fun _ -> Prims.l_True)
+
+/// Builds a tunnel.
+val impl_5__build (self: t_TunnelBuilder)
+    : Prims.Pure
+      (Core.Result.t_Result (Core.Pin.t_Pin (Alloc.Boxed.t_Box t_Tunnel Alloc.Alloc.t_Global))
+          (Sandwich.Error.t_Error & Sandwich.Tunnel.Io.t_BoxedIO))
+      Prims.l_True
+      (fun _ -> Prims.l_True)
