proofs/fstar/extraction/Sandwich.Implementation.Openssl3.Tunnel.Verify_callback.fsti
@@ -1,0 +1,125 @@
+module Sandwich.Implementation.Openssl3.Tunnel.Verify_callback
+#set-options "--fuel 0 --ifuel 1 --z3rlimit 15"
+open Core
+open FStar.Mul
+
+/// Returns the error stored in the X509 store context.
+val x509_store_context_get_error
+      (store_ctx: Core.Ptr.Non_null.t_NonNull Openssl3.t_x509_store_ctx_st)
+    : Prims.Pure i32 Prims.l_True (fun _ -> Prims.l_True)
+
+/// Returns the SSL object from a X509 store context.
+val x509_store_context_get_ssl (store_ctx: Core.Ptr.Non_null.t_NonNull Openssl3.t_x509_store_ctx_st)
+    : Prims.Pure (Core.Option.t_Option (Core.Ptr.Non_null.t_NonNull Openssl3.t_ssl_st))
+      Prims.l_True
+      (fun _ -> Prims.l_True)
+
+/// Records an error in the X509 store context.
+val x509_store_context_record_error
+      (#impl_765196419_: Type0)
+      {| i1: Core.Convert.t_Into impl_765196419_ i32 |}
+      (store_ctx: Core.Ptr.Non_null.t_NonNull Openssl3.t_x509_store_ctx_st)
+      (error: impl_765196419_)
+    : Prims.Pure Prims.unit Prims.l_True (fun _ -> Prims.l_True)
+
+(* item error backend: (reject_RawOrMutPointer) ExplicitRejection { reason: "a node of kind [Raw_pointer] have been found in the AST" }
+Last available AST for this item:
+
+/// The verify callback to be used.
+/// This callback is passed to `SSL_set_verify`.
+#[cfg(feature = "tunnel")]
+#[cfg(feature = "openssl3")]
+#[deny(bare_trait_objects)]
+#[feature(register_tool)]
+#[register_tool(_hax)]
+fn verify_callback(mut verify_code: int, store_ctx: raw_pointer!()) -> int {
+    {
+        let _: tuple0 = {
+            (if core::cmp::PartialEq::eq(verify_code, 1) {
+                rust_primitives::hax::never_to_any({ (return verify_code) })
+            })
+        };
+        (match (core::ptr::non_null::impl_3__new::<
+            openssl3::t_x509_store_ctx_st,
+        >(store_ctx)) {
+            core::option::Option_Some(store_ctx) => {
+                (match (sandwich::implementation::openssl3::tunnel::verify_callback::x509_store_context_get_ssl(
+                    store_ctx,
+                )) {
+                    core::option::Option_Some(ssl) => {
+                        let ssl_wrapped: sandwich::implementation::openssl3::tunnel::ssl::t_Ssl = {
+                            core::convert::f_from(ssl)
+                        };
+                        (match (sandwich::implementation::openssl3::tunnel::ssl::impl__Ssl__get_tunnel_security_requirements::<
+                            lifetime!(something),
+                        >(&(ssl_wrapped))) {
+                            core::option::Option_Some(security_requirements) => {
+                                let current_error: int = {
+                                    sandwich::implementation::openssl3::tunnel::verify_callback::x509_store_context_get_error(
+                                        store_ctx,
+                                    )
+                                };
+                                {
+                                    let _: tuple0 = {
+                                        (if sandwich::tunnel::tls::impl__TunnelSecurityRequirements__openssl3_assess_x509_store_error(
+                                            &(deref(security_requirements)),
+                                            current_error,
+                                        ) {
+                                            {
+                                                let _: tuple0 = { (verify_code = 1) };
+                                                {
+                                                    let _: tuple0 = {
+                                                        sandwich::implementation::openssl3::tunnel::verify_callback::x509_store_context_record_error::<
+                                                            int,
+                                                        >(store_ctx, cast(openssl3::v_X509_V_OK))
+                                                    };
+                                                    Tuple0
+                                                }
+                                            }
+                                        })
+                                    };
+                                    { verify_code }
+                                }
+                            }
+                            _ => {
+                                let _: rust_primitives::hax::t_Never = { (return 0) };
+                                Tuple0
+                            }
+                        })
+                    }
+                    _ => {
+                        let _: rust_primitives::hax::t_Never = { (return 0) };
+                        Tuple0
+                    }
+                })
+            }
+            _ => {
+                let _: rust_primitives::hax::t_Never = { (return 0) };
+                Tuple0
+            }
+        })
+    }
+}
+
+
+Last AST:
+/** print_rust: pitem: not implemented  (item: { Concrete_ident.T.def_id =
+  { Concrete_ident.Imported.krate = "sandwich";
+    path =
+    [{ Concrete_ident.Imported.data =
+       (Concrete_ident.Imported.TypeNs "implementation"); disambiguator = 0 };
+      { Concrete_ident.Imported.data =
+        (Concrete_ident.Imported.TypeNs "openssl3"); disambiguator = 0 };
+      { Concrete_ident.Imported.data =
+        (Concrete_ident.Imported.TypeNs "tunnel"); disambiguator = 0 };
+      { Concrete_ident.Imported.data =
+        (Concrete_ident.Imported.TypeNs "verify_callback"); disambiguator = 0
+        };
+      { Concrete_ident.Imported.data =
+        (Concrete_ident.Imported.ValueNs "verify_callback");
+        disambiguator = 0 }
+      ]
+    };
+  kind = Concrete_ident.Kind.Value }) */
+const _: () = ();
+ *)
