proofs/fstar/extraction/Sandwich.Io.Error.fsti
@@ -1,0 +1,68 @@
+module Sandwich.Io.Error
+#set-options "--fuel 0 --ifuel 1 --z3rlimit 15"
+open Core
+open FStar.Mul
+
+/// Types that can be converted to a [`pb::IOError`].
+class t_IntoIOError (v_Self: Type0) = {
+  f_into_io_error_pre:v_Self -> bool;
+  f_into_io_error_post:v_Self -> Sandwich_proto.Io.t_IOError -> bool;
+  f_into_io_error:x0: v_Self
+    -> Prims.Pure Sandwich_proto.Io.t_IOError
+        (f_into_io_error_pre x0)
+        (fun result -> f_into_io_error_post x0 result)
+}
+
+[@@ FStar.Tactics.Typeclasses.tcinstance]
+let impl: t_IntoIOError Std.Io.Error.t_ErrorKind =
+  {
+    f_into_io_error_pre = (fun (self: Std.Io.Error.t_ErrorKind) -> true);
+    f_into_io_error_post
+    =
+    (fun (self: Std.Io.Error.t_ErrorKind) (out: Sandwich_proto.Io.t_IOError) -> true);
+    f_into_io_error
+    =
+    fun (self: Std.Io.Error.t_ErrorKind) ->
+      match self with
+      | Std.Io.Error.ErrorKind_WouldBlock
+      | Std.Io.Error.ErrorKind_WriteZero
+      | Std.Io.Error.ErrorKind_Interrupted  ->
+        Sandwich_proto.Io.IOError_IOERROR_WOULD_BLOCK <: Sandwich_proto.Io.t_IOError
+      | Std.Io.Error.ErrorKind_NotConnected  ->
+        Sandwich_proto.Io.IOError_IOERROR_IN_PROGRESS <: Sandwich_proto.Io.t_IOError
+      | Std.Io.Error.ErrorKind_ConnectionRefused
+      | Std.Io.Error.ErrorKind_ConnectionReset
+      | Std.Io.Error.ErrorKind_ConnectionAborted
+      | Std.Io.Error.ErrorKind_TimedOut  ->
+        Sandwich_proto.Io.IOError_IOERROR_REFUSED <: Sandwich_proto.Io.t_IOError
+      | Std.Io.Error.ErrorKind_BrokenPipe  ->
+        Sandwich_proto.Io.IOError_IOERROR_CLOSED <: Sandwich_proto.Io.t_IOError
+      | Std.Io.Error.ErrorKind_NotFound
+      | Std.Io.Error.ErrorKind_PermissionDenied
+      | Std.Io.Error.ErrorKind_AlreadyExists
+      | Std.Io.Error.ErrorKind_InvalidInput
+      | Std.Io.Error.ErrorKind_InvalidData  ->
+        Sandwich_proto.Io.IOError_IOERROR_INVALID <: Sandwich_proto.Io.t_IOError
+      | Std.Io.Error.ErrorKind_Unsupported
+      | Std.Io.Error.ErrorKind_OutOfMemory  ->
+        Sandwich_proto.Io.IOError_IOERROR_SYSTEM_ERROR <: Sandwich_proto.Io.t_IOError
+      | Std.Io.Error.ErrorKind_AddrInUse
+      | Std.Io.Error.ErrorKind_AddrNotAvailable  ->
+        Sandwich_proto.Io.IOError_IOERROR_ADDRESS_IN_USE <: Sandwich_proto.Io.t_IOError
+      | _ -> Sandwich_proto.Io.IOError_IOERROR_UNKNOWN <: Sandwich_proto.Io.t_IOError
+  }
+
+[@@ FStar.Tactics.Typeclasses.tcinstance]
+let impl_1: t_IntoIOError Std.Io.Error.t_Error =
+  {
+    f_into_io_error_pre = (fun (self: Std.Io.Error.t_Error) -> true);
+    f_into_io_error_post
+    =
+    (fun (self: Std.Io.Error.t_Error) (out: Sandwich_proto.Io.t_IOError) -> true);
+    f_into_io_error
+    =
+    fun (self: Std.Io.Error.t_Error) ->
+      f_into_io_error #Std.Io.Error.t_ErrorKind
+        #FStar.Tactics.Typeclasses.solve
+        (Std.Io.Error.impl__Error__kind self <: Std.Io.Error.t_ErrorKind)
+  }
