proofs/fstar/extraction/Sandwich.Io.fsti
@@ -1,0 +1,27 @@
+module Sandwich.Io
+#set-options "--fuel 0 --ifuel 1 --z3rlimit 15"
+open Core
+open FStar.Mul
+
+let _ =
+  (* This module has implicit dependencies, here we make them explicit. *)
+  (* The implicit dependencies arise from typeclasses instances. *)
+  let open Std.Io in
+  ()
+
+/// An IO interface that implements both [`Read`] and [`Write`] traits.
+class t_IO (v_Self: Type0) = {
+  [@@@ FStar.Tactics.Typeclasses.no_method]_super_4807793307859852082:Std.Io.t_Read v_Self;
+  [@@@ FStar.Tactics.Typeclasses.no_method]_super_7415520646860052681:Std.Io.t_Write v_Self
+}
+
+[@@ FStar.Tactics.Typeclasses.tcinstance]
+let impl
+      (#v_T: Type0)
+      (#[FStar.Tactics.Typeclasses.tcresolve ()] i1: Std.Io.t_Read v_T)
+      (#[FStar.Tactics.Typeclasses.tcresolve ()] i2: Std.Io.t_Write v_T)
+    : t_IO v_T =
+  {
+    _super_4807793307859852082 = FStar.Tactics.Typeclasses.solve;
+    _super_7415520646860052681 = FStar.Tactics.Typeclasses.solve
+  }
