proofs/fstar/extraction/Sandwich.Support.fsti
@@ -4,5 +4,5 @@ open Core
 open FStar.Mul
 
 /// Checks if a given string contains any of the characters from another string.
-val contains_any_of (v_string invalid_chars: string)
-    : Prims.Pure bool Prims.l_True (fun _ -> Prims.l_True)
+/// NOTE: renamed the input "string" to "s" to avoid a type name clash in F*
+val contains_any_of (s invalid_chars: string) : Prims.Pure bool Prims.l_True (fun _ -> Prims.l_True)
